

$$\begin{bmatrix} \ddot{\phi} \\ \ddot{p} \end{bmatrix} = \begin{bmatrix} 0 & 1 \\ -k_{\phi}/I_x & -k_p/I_x \end{bmatrix} \quad \begin{bmatrix} \ddot{\theta} \\ \ddot{q} \end{bmatrix} = \begin{bmatrix} 0 & 1 \\ -k_{\theta}/I_y & -k_q/I_y \end{bmatrix}$$

$$k_p = -(\lambda_1 + \lambda_2)I_x \quad k_{\phi} = \lambda_1 \lambda_2 I_x \quad k_r = 0.004 \text{ from 2.3}$$

$$k_q = -(\lambda_1 + \lambda_2)I_y \quad k_{\theta} = \lambda_1 \lambda_2 I_y$$

$$\lambda_1 = -1/\tau \rightarrow \tau = 0.5, \lambda_1 = -2$$

$$\lambda_2 < \lambda_1 \text{ so } \lambda_1 \text{ dominates, ex: } \lambda_2 = -10$$

$$\text{for } \lambda_1 = -2, \lambda_2 = -10, I_x = 5.8 \cdot 10^{-5} \text{ kg} \cdot \text{m}^2, I_y = 7.2 \cdot 10^{-5} \text{ kg} \cdot \text{m}^2$$

$$k_p = 0.000696 \quad k_{\phi} = 0.00116 \quad k_q = 0.000864 \quad k_{\theta} = 0.00141$$

$(k_{1x}) \quad \quad \quad (k_{2x}) \quad \quad \quad (k_{1y}) \quad \quad \quad (k_{2y})$

$$L = -k_{\phi}\phi - k_p p \quad M = -k_{\theta}\theta - k_q q \quad N = -k_r r$$

$$L = -0.00116\phi - 0.000696p$$

$$M = -0.00141\theta - 0.000864q$$

$$N = -0.004r$$